CCsub_Subcapt.v
@@ -92,23 +92,19 @@ Qed.
 
 Lemma wf_store_cse_no_fvar: forall S x R T l,
   wf_store_ctx S ->
-  Store.binds l (R # T) S ->
-  x `notin` `cse_fvars` R.
+  StoreImpl.binds l (R # T) S ->
+  x `notin`A `cse_fvars` R.
 Proof with eauto.
   intros * WfS HBinds.
   induction WfS...
-  - inversion HBinds.
-  - Store.binds_cases HBinds.
-    + apply (IHWfS H1).
-    + inversion H3. subst.
-      inversion H; subst.
-      inversion H4; subst...
-      -- inversion H1.
-      -- apply wf_cse_fvars_from_ctx in H4.
-         fsetdec.
+  StoreImpl.analyze_binds HBinds...
+  inversion select (_ = _); subst...
+  inversion H; subst...
+  intro.
+  apply wf_cse_fvars_from_ctx with (x := x) in H3...
+  fsetdec.
 Qed.
 
-(* Needed, line 664 *)
 (* Substituting the same capture set preserves subcapturing *)
 Lemma subcapt_through_subst_cse : forall x D Q C Δ Γ S C1 C2 ,
   subcapt (Δ ++ [(x, bind_typ (D # Q))] ++ Γ) S C1 C2 ->
@@ -128,16 +124,10 @@ Proof with eauto using wf_ctx_subst_cb, wf_cse_subst_cb with fsetdec.
     destruct (x == X).
     + apply subcapt_reflexivity... apply wf_cse_weaken_head...
     + apply subcapt_reflexivity... inversion H0. subst.
-      binds_cases H4.
-      * eauto.
-      * econstructor.
-        assert (binds X (bind_typ T0) (G ++ Γ)). {
-          apply binds_head...
-        }
-        assert (binds X (subst_cb x C (bind_typ T0)) (map (subst_cb x C) G ++ Γ)).
-        { apply (binds_map binding binding X (bind_typ T0) (subst_cb x C) (G ++ Γ)) in H1.
-          auto. }
-        apply H3.
+      analyze_binds H4...
+      econstructor.
+      assert (binds X (bind_typ T0) (G ++ Γ)) by (apply binds_app_2; eauto).
+      assert (binds X (subst_cb x C (bind_typ T0)) (map (subst_cb x C) G ++ Γ))...
   - constructor...
     apply (wf_cse_subst_cb Γ G (D # T) x (cse_loc l) C S)...
   - destruct (x == X).
@@ -145,64 +135,53 @@ Proof with eauto using wf_ctx_subst_cb, wf_cse_subst_cb with fsetdec.
       eapply (subcapt_transitivity (map (subst_cb X C) G ++ Γ) S C D (subst_cse X C Q)).
       * rewrite_env (nil ++ (map (subst_cb X C) G ++ Γ)).
         apply subcapt_weakening...
-        eapply wf_ctx_subst_cb. apply subcapt_regular in C1subC2.
-        destruct C1subC2 as [WfS [WfCtx _]]. apply WfCtx. apply subcapt_regular in CsubD.
-        destruct CsubD as [_ [_ [H3 _]]]...
       * rewrite (subst_cse_fresh X D C).
-        -- binds_cases H.
-        ++ simpl in Fr0. fsetdec. (* X in Γ *)
-        ++ inversion H0. subst. apply IHC1subC2... (* X in [(X, bind_typ (D # T))] *)
-        ++ (* X in G, contradiciton, environment is not ok *)
+        -- analyze_binds_uniq H...
+           (* X in G, contradiciton, environment is not ok *)
            assert (wf_ctx (G ++ [(X, bind_typ (D # T))] ++ Γ) S) as HCtx.
            { apply subcapt_regular in C1subC2. destruct C1subC2 as [_ [hwf _]]... }
-           apply ok_from_wf_ctx in HCtx.
+           apply uniq_from_wf_ctx in HCtx.
            apply fresh_mid_head in HCtx.
-           apply binds_In in H1.
-           unfold not in HCtx. apply HCtx in H1. inversion H1.
+           inversion BindsTacVal; subst...
         -- apply (notin_fv_wf_cse Γ) with (S := S).
-          ++ apply subcapt_regular in CsubD. destruct CsubD as [_ [_ [_ Dwf]]]...
-          ++ assert (wf_ctx (G ++ [(X, bind_typ (D # T))] ++ Γ) S).
-             { apply subcapt_regular in C1subC2. destruct C1subC2 as [_ [hwf _]]... }
-             apply ok_from_wf_ctx in H0.
-             apply fresh_mid_tail in H0. assumption.
-    + binds_cases H.
-      * apply (subcapt_trans_var (subst_cse x C R) S (map (subst_cb x C) G ++ Γ) (subst_cse x C Q) X (subst_ct x C T0)).
-        -- apply binds_tail.
-          ++ rewrite (map_subst_cb_id Γ x C S).
-             apply binds_map with (f:=(subst_cb x C)) in H. simpl in H...
-             apply subcapt_regular in CsubD. destruct CsubD...
-             apply subcapt_regular in C1subC2. destruct C1subC2 as [_ [HCtx _]].
-             apply ok_from_wf_ctx in HCtx. apply fresh_mid_tail in HCtx... 
-          ++ rewrite dom_map...
-        -- apply IHC1subC2... 
+           ++ apply subcapt_regular in CsubD. destruct CsubD as [_ [_ [_ Dwf]]]...
+           ++ assert (wf_ctx (G ++ [(X, bind_typ (D # T))] ++ Γ) S).
+              { apply subcapt_regular in C1subC2. destruct C1subC2 as [_ [hwf _]]... }
+              apply uniq_from_wf_ctx in H0.
+              apply fresh_mid_tail in H0. assumption.
+    + analyze_binds H...
       * assert (subcapt (map (subst_cb x C) G ++ Γ) S (cse_fvar X) (subst_cse x C R)).
         { apply (subcapt_trans_var (subst_cse x C R) S (map (subst_cb x C) G ++ Γ) (subst_cse x C R) X (subst_ct x C T0)).
-          - assert (HH := H1).
-            apply binds_map with (f:=(subst_cb x C)) in H1. simpl in H1.
+          - assert (HH := BindsTac).
+            apply binds_map with (f:=(subst_cb x C)) in BindsTac. simpl in BindsTac.
             apply subcapt_regular in C1subC2. destruct C1subC2 as [_ [HCtx _]].
-            apply ok_from_wf_ctx in HCtx. apply ok_remove_mid in HCtx.
-            apply binds_head with (E:=Γ) in H1...
+            apply uniq_from_wf_ctx in HCtx. apply uniq_remove_mid in HCtx.
+            apply binds_app_2 with (F:=Γ) in BindsTac...
           - assert (HH := IHC1subC2 CsubD G ltac:(fsetdec)).
             apply subcapt_regular in HH. destruct HH as [HH1 [HH2 [HH3 HH4]]].
             apply subcapt_reflexivity.
             auto. auto.
         }
         eapply subcapt_transitivity. apply H. apply IHC1subC2...
+      * apply (subcapt_trans_var (subst_cse x C R) S (map (subst_cb x C) G ++ Γ) (subst_cse x C Q) X (subst_ct x C T0)).
+        -- apply binds_app_3.
+           rewrite (map_subst_cb_id Γ x C S).
+           apply binds_map with (f:=(subst_cb x C)) in BindsTac0. simpl in BindsTac0...
+           apply subcapt_regular in CsubD. destruct CsubD...
+           apply subcapt_regular in C1subC2. destruct C1subC2 as [_ [HCtx _]].
+           apply uniq_from_wf_ctx in HCtx. apply fresh_mid_tail in HCtx... 
+        -- apply IHC1subC2... 
   - specialize (IHC1subC2 CsubD G ltac:(fsetdec)).
     epose proof (subcapt_regular _ _ _ _ CsubD) as [WfS [WfCtx [WfC _]]].
     epose proof (subcapt_regular _ _ _ _ C1subC2) as [_ [WfCtx2 _]].
     epose proof (wf_store_cse_no_fvar _ x _ _ _ WfS H) as HR.
-    assert (subcapt (map (subst_cb x C) G ++ Γ) S (cse_loc X) (subst_cse x C R)). {
+    assert (subcapt (map (subst_cb x C) G ++ Γ) S (cse_loc l) (subst_cse x C R)). {
       apply subcapt_trans_loc with (R := R) (T := T0)...
       rewrite <- (subst_cse_fresh x R C)...
       apply subcapt_reflexivity...
-      epose proof (wf_pair_from_wf_store_ctx nil S R T0 X WfS ltac:(constructor) H) as [WfR _]...
+      epose proof (wf_pair_from_wf_store_ctx nil S R T0 l WfS ltac:(constructor) H) as [WfR _]...
       rewrite_env ((map (subst_cb x C) G ++ Γ) ++ nil).
       apply wf_cse_weaken_head with (Δ := (map (subst_cb x C) G ++ Γ))...
-      simpl_env.
-      apply ok_from_wf_ctx in WfCtx2.
-      apply ok_remove_mid in WfCtx2.
-      apply ok_map_app_l with (f := (subst_cb x C)) in WfCtx2...
     }
     eapply subcapt_transitivity with (Q := (subst_cse x C R)) ...
   - constructor...
@@ -255,16 +234,13 @@ Proof with simpl_env; eauto.
     try apply H0; try apply WfCtx; apply sub_regular in PsubQ;
     destruct PsubQ as [subwf1 [subwf2 [subwf3 subwf4]]]; auto; auto).
   - apply (subcapt_trans_var R S (map (subst_tb Z P) G ++ E) Q0 X (subst_tt Z P T))...
-    binds_cases H. 
-    + (* X in E *)
-      apply binds_tail. eapply binds_map with (f := subst_tb Z P) in H. simpl in H.
-      erewrite <- map_subst_tb_id in H. apply H. eauto.
-      apply binding_uniq_from_wf_ctx in WfCtx. auto.
-      apply binding_uniq_from_wf_ctx in WfCtx. auto.
-    + (* X in G *)
-      apply binds_head.
-      eapply binds_map with (f := subst_tb Z P) in H1. simpl in H1.
-      apply H1.
+    analyze_binds_uniq H...
+    + apply binds_app_2.
+      eapply binds_map with (f := subst_tb Z P) in BindsTac. simpl in BindsTac...
+    + apply binds_app_3.
+      eapply binds_map with (f := subst_tb Z P) in BindsTac0. simpl in BindsTac0.
+      erewrite <- map_subst_tb_id in BindsTac0...
+      apply binding_uniq_from_wf_ctx in WfCtx...
   - apply subcapt_join_inl; auto.
     eapply wf_cse_subst_tb.
     apply H. apply sub_regular in PsubQ as [_ [_ [Pwf _]]]...
