Meta/MetatheoryLoc.v
@@ -1,0 +1,286 @@
+(* This file is distributed under the terms of the MIT License, also
+   known as the X11 Licence.  A copy of this license is in the README
+   file that accompanied the original distribution of this file.
+
+   Based on code written by:
+     Brian Aydemir
+     Arthur Charg\'eraud *)
+
+Require Import Coq.Arith.Arith.
+Require Import Coq.Classes.EquivDec.
+Require Import Coq.Lists.List.
+Require Import Coq.Structures.Equalities.
+
+Require Import Coq.FSets.FSets.
+Require Import CoqListFacts.
+Require Import FSetExtra.
+Require Import FSetWeakNotin.
+Require Import LibTactics.
+
+Require Import Lia.
+
+(* ********************************************************************** *)
+(** * Defining locs *)
+
+(** Locs are structureless objects such that we can always generate
+    one fresh from a finite collection.  Equality on locs is [eq] and
+    decidable.  We use Coq's module system to make abstract the
+    implementation of locs. *)
+
+Module Type LOC <: UsualDecidableType.
+
+  Parameter loc : Set.
+  Definition t := loc.
+
+  Parameter eq_dec : forall x y : loc, {x = y} + {x <> y}.
+
+  Parameter loc_fresh_for_list :
+    forall (xs : list t), {x : loc | ~ List.In x xs}.
+
+  Parameter fresh : list loc -> loc.
+
+  Parameter fresh_not_in : forall l, ~ In (fresh l) l.
+
+  Parameter nat_of : loc -> nat.
+
+  #[global]
+  Hint Resolve eq_dec : core.
+
+  Include HasUsualEq <+ UsualIsEq <+ UsualIsEqOrig.
+
+End LOC.
+
+(** The implementation of the above interface is hidden for
+    documentation purposes. *)
+
+Module Loc : LOC.
+
+  (* begin hide *)
+  Definition loc := nat.
+  Definition t := loc.
+
+  Definition eq_dec := eq_nat_dec.
+
+  Lemma max_lt_r : forall x y z,
+    x <= z -> x <= max y z.
+  Proof.
+    induction x. auto with arith.
+    induction y. auto with arith.
+      simpl. induction z. lia. auto with arith.
+  Qed.
+
+  Lemma nat_list_max : forall (xs : list nat),
+    { n : nat | forall x, List.In x xs -> x <= n }.
+  Proof.
+    induction xs as [ | x xs [y H] ].
+    (* case: nil *)
+    exists 0. inversion 1.
+    (* case: cons x xs *)
+    exists (max x y). intros z J. simpl in J. destruct J as [K | K].
+      subst. auto with arith.
+      auto using max_lt_r.
+  Qed.
+
+  Lemma loc_fresh_for_list :
+    forall (xs : list nat), { n : nat | ~ List.In n xs }.
+  Proof.
+    intros xs. destruct (nat_list_max xs) as [x H].
+    exists (S x). intros J. lapply (H (S x)). lia. trivial.
+  Qed.
+
+  Definition fresh (l : list loc) :=
+    match loc_fresh_for_list l with
+      (exist _ x _) => x
+    end.
+
+  Lemma fresh_not_in : forall l, ~ In (fresh l) l.
+  Proof.
+    intro l. unfold fresh.
+    destruct loc_fresh_for_list. auto.
+  Qed.
+
+  Definition nat_of := fun (x : loc) => x.
+
+  Include HasUsualEq <+ UsualIsEq <+ UsualIsEqOrig.
+
+  (* end hide *)
+
+End Loc.
+
+(** We make [loc], [fresh], [fresh_not_in] and [loc_fresh_for_list] available
+    without qualification. *)
+
+Notation loc := Loc.loc.
+Notation fresh := Loc.fresh.
+Notation fresh_not_in := Loc.fresh_not_in.
+Notation loc_fresh_for_list := Loc.loc_fresh_for_list.
+
+(* Automatically unfold Loc.eq *)
+Global Arguments Loc.eq /.
+
+(** It is trivial to declare an instance of [EqDec] for [loc]. *)
+
+#[export] Instance EqDec_loc : @EqDec loc eq eq_equivalence.
+Proof. exact Loc.eq_dec. Defined.
+
+
+(* ********************************************************************** *)
+(** * Finite sets of locs *)
+
+(** We use our implementation of locs to obtain an implementation of
+    finite sets of locs.  We give the resulting type an intuitive
+    name, as well as import names of set operations for use within
+    this library.  In order to avoid polluting Coq's namespace, we do
+    not use [Module Export]. *)
+
+Module Import LocSetImpl : FSetExtra.WSfun Loc :=
+  FSetExtra.Make Loc.
+
+Notation locs :=
+  LocSetImpl.t.
+
+(** The [LocSetDecide] module provides the [fsetdec] tactic for
+    solving facts about finite sets of locs. *)
+
+
+Module Export LocSetDecide := Coq.FSets.FSetDecide.WDecide_fun Loc LocSetImpl.
+
+(** The [LocSetNotin] module provides the [destruct_notin] and
+    [solve_notin] for reasoning about non-membership in finite sets of
+    locs, as well as a variety of lemmas about non-membership. *)
+
+Module Export LocSetNotin := FSetWeakNotin.Notin_fun Loc LocSetImpl.
+
+(** Given the [fsetdec] tactic, we typically do not need to refer to
+    specific lemmas about finite sets.  However, instantiating
+    functors from the FSets library makes a number of setoid rewrites
+    available.  These rewrites are crucial to developments since they
+    allow us to replace a set with an extensionally equal set (see the
+    [Equal] relation on finite sets) in propositions about finite
+    sets. *)
+
+Module LocSetFacts := FSetFacts.WFacts_fun Loc LocSetImpl.
+Module LocSetProperties := FSetProperties.WProperties_fun Loc LocSetImpl.
+
+Export LocSetFacts.
+
+(* ********************************************************************** *)
+(** * Properties *)
+
+(** For any given finite set of locs, we can generate an loc fresh
+    for it. *)
+
+Lemma loc_fresh : forall L : locs, { x : loc | ~ In x L }.
+Proof.
+  intros L. destruct (loc_fresh_for_list (elements L)) as [a H].
+  exists a. intros J. contradiction H.
+  rewrite <- CoqListFacts.InA_iff_In. auto using elements_1.
+Qed.
+
+
+(* ********************************************************************** *)
+(** * Tactic support for picking fresh locs *)
+
+(* begin hide *)
+
+(** The auxiliary tactic [simplify_list_of_loc_sets] takes a list of
+    finite sets of locs and unions everything together, returning the
+    resulting single finite set. *)
+
+Ltac simplify_list_of_loc_sets L :=
+  let L := eval simpl in L in
+  let L := ltac_remove_dups L in
+  let L := eval simpl in (List.fold_right union empty L) in
+  match L with
+    | context C [union ?E empty] => context C [ E ]
+  end.
+
+(* end hide *)
+
+(** [gather_locs_with F] returns the union of all the finite sets
+    [F x] where [x] is a variable from the context such that [F x]
+    type checks. *)
+
+Ltac gather_locs_with F :=
+  let apply_arg x :=
+    match type of F with
+      | _ -> _ -> _ -> _ => constr:(@F _ _ x)
+      | _ -> _ -> _ => constr:(@F _ x)
+      | _ -> _ => constr:(@F x)
+    end in
+  let rec gather V :=
+    match goal with
+      | H : _ |- _ =>
+        let FH := apply_arg H in
+        match V with
+          | context [FH] => fail 1
+          | _ => gather (union FH V)
+        end
+      | _ => V
+    end in
+  let L := gather empty in eval simpl in L.
+
+(** [beautify_fset V] assumes that [V] is built as a union of finite
+    sets and returns the same set cleaned up: empty sets are removed
+    and items are laid out in a nicely parenthesized way. *)
+
+Ltac beautify_fset V :=
+  let rec go Acc E :=
+     match E with
+     | union ?E1 ?E2 => let Acc2 := go Acc E2 in go Acc2 E1
+     | empty => Acc
+     | ?E1 => match Acc with
+                | empty => E1
+                | _ => constr:(union E1 Acc)
+              end
+     end
+  in go empty V.
+
+(** The tactic [pick fresh Y for L] takes a finite set of locs [L]
+    and a fresh name [Y], and adds to the context an loc with name
+    [Y] and a proof that [~ In Y L], i.e., that [Y] is fresh for [L].
+    The tactic will fail if [Y] is already declared in the context.
+
+    The variant [pick fresh Y] is similar, except that [Y] is fresh
+    for "all locs in the context."  This version depends on the
+    tactic [gather_locs], which is responsible for returning the set
+    of "all locs in the context."  By default, it returns the empty
+    set, but users are free (and expected) to redefine it. *)
+
+Ltac gather_locs :=
+  constr:(empty).
+
+Tactic Notation "pick" "lfresh" ident(Y) "for" constr(L) :=
+  let Fr := fresh "Fr" in
+  let L := beautify_fset L in
+  (destruct (loc_fresh L) as [Y Fr]).
+
+Tactic Notation "pick" "lfresh" ident(Y) :=
+  let L := gather_locs in
+  pick lfresh Y for L.
+
+Ltac pick_lfresh y :=
+  pick lfresh y.
+
+(** Example: We can redefine [gather_locs] to return all the
+    "obvious" locs in the context using the [gather_locs_with] thus
+    giving us a "useful" version of the "[pick lfresh]" tactic. *)
+
+Ltac gather_locs ::=
+  let A := gather_locs_with (fun x : locs => x) in
+  let B := gather_locs_with (fun x : loc => singleton x) in
+  constr:(union A B).
+
+Lemma example_pick_lfresh_use : forall (x y z : loc) (L1 L2 L3: locs), True.
+(* begin show *)
+Proof.
+  intros x y z L1 L2 L3.
+  pick_lfresh k.
+
+  (** At this point in the proof, we have a new loc [k] and a
+      hypothesis [Fr] that [k] is fresh for [x], [y], [z], [L1], [L2],
+      and [L3]. *)
+
+  trivial.
+Qed.
+(* end show *)
