MetatheoryExtras.v
@@ -1,0 +1,74 @@
+Require Import Metatheory.
+Require Import AssocList.
+
+Tactic Notation
+    "pick" "fresh" ident(atom_name)
+    "excluding" constr(L)
+    "and" "destruct" constr(H) :=
+  let L := beautify_fset L in
+  pick fresh atom_name for L;
+  first [ destruct (@H atom_name ltac:(fsetdec))
+        | edestruct (@H atom_name ltac:(fsetdec))].
+
+Tactic Notation
+    "pick" "fresh" ident(atom_name)
+    "excluding" constr(L)
+    "and" "destruct" constr(H) "as" simple_intropattern(pat) :=
+  let L := beautify_fset L in
+  pick fresh atom_name for L;
+  first [ destruct (@H atom_name ltac:(fsetdec)) as pat
+        | edestruct (@H atom_name ltac:(fsetdec)) as pat].
+
+Tactic Notation
+    "pick" "fresh" ident(atom_name)
+    "excluding" constr(L)
+    "and" "specialize" constr(H) :=
+  let L := beautify_fset L in
+  pick fresh atom_name for L;
+  specialize (@H atom_name ltac:(fsetdec)).
+
+Notation "E `subset`A F" :=
+  (AtomSetImpl.Subset E F)
+  (at level 68)
+  : set_scope.
+
+Ltac notin_simpl := AtomSetNotin.destruct_notin.
+Ltac notin_solve := AtomSetNotin.solve_notin.
+Ltac lnotin_simpl := LocSetNotin.destruct_notin.
+
+Lemma atomset_subset_union : forall A1 A2 B1 B2,
+  AtomSetImpl.Subset A1 A2 ->
+  AtomSetImpl.Subset B1 B2 ->
+  AtomSetImpl.Subset (AtomSetImpl.union A1 B1) (AtomSetImpl.union A2 B2).
+Proof.
+  intros.
+  fsetdec.
+Qed.
+
+Lemma binds_remove_mid_cons :
+  forall (A : Type) (x y : atom) (a b : A) (F G : list (atom * A)),
+  binds x a (F ++ (y, b) :: G) -> x <> y -> binds x a (F ++ G).
+Proof. intros *. clear. intros H. analyze_binds H. Qed.
+
+Lemma fresh_mid : 
+  forall (A : Type) (x : atom) (a : A) (E F : list (atom * A)),
+  uniq (F ++ x ~ a ++ E) -> x `notin`A union (dom F) (dom E).
+Proof. intros *. clear. solve_uniq. Qed.
+
+Lemma nil_concat : forall (A: Type) (E: list (atom * A)),
+  nil ++ E = E.
+Proof.
+  reflexivity.
+Qed.
+
+Ltac rewrite_nil_concat :=
+  match goal with
+  | |- _ ?E0 =>
+    rewrite <- nil_concat with (E := E0)
+  | |- _ ?E0 _ =>
+    rewrite <- nil_concat with (E := E0)
+  | |- _ ?E0 _ _ =>
+    rewrite <- nil_concat with (E := E0)
+  | |- _ ?E0 _ _ _ =>
+    rewrite <- nil_concat with (E := E0)
+  end.
